Rewrite properties of STLC by using Autosubst.

stlc/Constraint.v
@@ -1,5 +1,6 @@
+Require Import Autosubst.Autosubst.
 Require Import List Recdef Omega.
-Require Id Types.
+Require VarSet Types.
 
 Lemma Forall_map : forall X Y (P : Y -> Prop) (f : X -> Y) l,
   Forall P (map f l) <-> Forall (fun x => P (f x)) l.
@@ -11,58 +12,58 @@ Qed.
 Definition t := list (Types.t * Types.t).
 
 Notation FV c :=
-  (fold_right Id.FSet.union Id.FSet.empty
-    (map (fun p => Id.FSet.union (Types.FV (fst p)) (Types.FV (snd p))) c)).
+  (fold_right VarSet.union VarSet.empty
+    (map (fun p => VarSet.union (Types.FV (fst p)) (Types.FV (snd p))) c)).
 
 Notation size c :=
   (fold_right plus 0 (map (fun p =>
     Types.size (fst p) + Types.size (snd p)) c)).
 
-Notation subst s c :=
-  (map (fun p => (Types.subst s (fst p), Types.subst s (snd p))) c).
+Instance HSubst_t : HSubst Types.t t :=
+  fun sigma c => map (fun p => (subst sigma (fst p), subst sigma (snd p))) c.
 
 Notation unifies s c :=
-  (Forall (fun p => Types.subst s (fst p) = Types.subst s (snd p)) c).
+  (Forall (fun p => (fst p).[s] = (snd p).[s]) c).
 
 Lemma subst_FV : forall x s c,
-  Id.FSet.In x (FV (subst s c)) ->
-  exists y, Id.FSet.In x (Types.FV (s y)) /\ Id.FSet.In y (FV c).
+  VarSet.In x (FV (c.|[s])) ->
+  exists y, VarSet.In x (Types.FV (s y)) /\ VarSet.In y (FV c).
 Proof.
   intros ? ? c H.
   induction c as [| [] ]; simpl in *.
-  - destruct (Id.FSet.empty_spec H).
-  - apply Id.FSet.union_spec in H.
+  - destruct (VarSet.empty_spec H).
+  - apply VarSet.union_spec in H.
     destruct H as [ H | H ].
-    + apply Id.FSet.union_spec in H.
+    + apply VarSet.union_spec in H.
       destruct H as [H | H];
       destruct (Types.subst_FV _ _ _ H) as [? []]; eauto 7.
     + destruct (IHc H) as [? []]; eauto.
 Qed.
 
 Definition lt c1 c2 :=
-  (Id.FSet.cardinal (FV c1) <= Id.FSet.cardinal (FV c2)) /\
-  (Id.FSet.cardinal (FV c2) <= Id.FSet.cardinal (FV c1) -> size c1 < size c2).
+  (VarSet.cardinal (FV c1) <= VarSet.cardinal (FV c2)) /\
+  (VarSet.cardinal (FV c2) <= VarSet.cardinal (FV c1) -> size c1 < size c2).
 
 Lemma lt_subst : forall c x t t1 t2,
-  ~Id.FSet.In x (Types.FV t) ->
+  ~VarSet.In x (Types.FV t) ->
   (t1 = t /\ t2 = Types.Var x \/ t1 = Types.Var x /\ t2 = t) ->
-  lt (subst (Types.subst_single x t) c) ((t1, t2) :: c).
+  lt (c.|[Types.subst_single x t]) ((t1, t2) :: c).
 Proof.
   intros c x t ? ? Hmem Heq.
-  assert (Hcardinal : Id.FSet.cardinal (FV (subst (Types.subst_single x t) c)) < Id.FSet.cardinal (FV ((t1, t2) :: c))).
-  - apply Id.FSetProperties.subset_cardinal_lt with (x := x); simpl.
+  assert (Hcardinal : VarSet.cardinal (FV c.|[Types.subst_single x t]) < VarSet.cardinal (FV ((t1, t2) :: c))).
+  - apply VarSet.subset_cardinal_lt with (x := x); simpl.
     + intros y HIn.
       destruct (subst_FV _ _ _ HIn) as [z [H]].
       unfold Types.subst_single in *.
-      destruct (Id.eq_dec x z);
-      [| apply Id.FSet.singleton_spec in H ];
+      destruct (Nat.eq_dec x z);
+      [| apply VarSet.singleton_spec in H ];
       destruct Heq as [[] | []]; subst; simpl in *; eauto.
     + destruct Heq as [[] | []]; subst; simpl; eauto 6.
     + intros Hoccur.
       destruct (subst_FV _ _ _ Hoccur) as [z [H]].
       unfold Types.subst_single in *.
-      destruct (Id.eq_dec x z);
-      [| apply Id.FSet.singleton_spec in H ];
+      destruct (Nat.eq_dec x z);
+      [| apply VarSet.singleton_spec in H ];
       subst; eauto.
   - split; omega.
 Qed.
@@ -72,7 +73,7 @@ Lemma lt_cons : forall p c,
 Proof.
   intros [t] c.
   split; simpl in *.
-  - apply Id.FSetProperties.subset_cardinal.
+  - apply VarSet.subset_cardinal.
     intros ? ?.
     eauto.
   - specialize (Types.size_gt_0 t). intros. omega.
@@ -84,15 +85,15 @@ Lemma lt_fun : forall t11 t12 t21 t22 c',
 Proof.
   intros.
   split; simpl.
-  - apply Id.FSetProperties.subset_cardinal.
+  - apply VarSet.subset_cardinal.
     intros ? H.
-    apply Id.FSet.union_spec in H.
+    apply VarSet.union_spec in H.
     destruct H as [ H | H ].
-    + apply Id.FSet.union_spec in H.
+    + apply VarSet.union_spec in H.
       destruct H; eauto 7.
-    + apply Id.FSet.union_spec in H.
+    + apply VarSet.union_spec in H.
       destruct H as [ H | H ].
-      * apply Id.FSet.union_spec in H.
+      * apply VarSet.union_spec in H.
         destruct H; eauto 7.
       * eauto.
   - omega.
@@ -103,7 +104,7 @@ Hint Resolve lt_subst lt_cons lt_fun.
 Lemma lt_wf : well_founded lt.
 Proof.
   intros c.
-  remember (Id.FSet.cardinal (FV c)) as n.
+  remember (VarSet.cardinal (FV c)) as n.
   generalize dependent c.
   induction n as [n IHn] using lt_wf_ind.
   intros.
@@ -112,7 +113,7 @@ Proof.
   constructor.
   intros c' Hlt.
   destruct Hlt as [ ? Hlt ].
-  destruct (eq_nat_dec (Id.FSet.cardinal (FV c)) (Id.FSet.cardinal (FV c'))).
+  destruct (eq_nat_dec (VarSet.cardinal (FV c)) (VarSet.cardinal (FV c'))).
   - apply IHc; eauto.
     apply Hlt.
     omega.
@@ -128,34 +129,30 @@ Function unify_aux c { wf lt c } :=
       else
         match t1, t2 with
         | Types.Var x, _ =>
-            if Id.FSet.mem x (Types.FV t2) then None
-            else option_map (cons (x, t2)) (unify_aux (subst (Types.subst_single x t2) c'))
+            if VarSet.mem x (Types.FV t2) then None
+            else option_map (cons (x, t2)) (unify_aux (c'.|[Types.subst_single x t2]))
         | _, Types.Var x =>
-            if Id.FSet.mem x (Types.FV t1) then None
-            else option_map (cons (x, t1)) (unify_aux (subst (Types.subst_single x t1) c'))
+            if VarSet.mem x (Types.FV t1) then None
+            else option_map (cons (x, t1)) (unify_aux (c'.|[Types.subst_single x t1]))
         | Types.Fun t11 t12, Types.Fun t21 t22 =>
             unify_aux ((t11, t21) :: (t12, t22) :: c')
-        | _, _ => None
         end
   end.
 Proof.
   - intros. eauto.
-  - intros. apply lt_subst; eauto.
-    apply Id.FSetProperties.Dec.F.not_mem_iff.
-    eauto.
   - intros. eauto.
   - intros. apply lt_subst; eauto.
-    apply Id.FSetProperties.Dec.F.not_mem_iff.
+    apply VarSet.Dec.F.not_mem_iff.
     eauto.
   - intros. apply lt_subst; eauto.
-    apply Id.FSetProperties.Dec.F.not_mem_iff.
+    apply VarSet.Dec.F.not_mem_iff.
     eauto.
   - apply lt_wf.
 Qed.
 
 Definition unify c :=
   option_map (fold_right
-    (fun p s x => Types.subst s (Types.subst_single (fst p) (snd p) x))
+    (fun p s x => (Types.subst_single (fst p) (snd p) x).[s])
     Types.Var) (unify_aux c).
 
 Theorem unify_sound : forall c s,
@@ -173,13 +170,13 @@ Proof.
       eauto.
     + destruct t1; destruct t2;
         repeat match goal with
-        | H : context [if Id.FSet.mem ?x ?s then _ else _] |- _ =>
+        | H : context [if VarSet.mem ?x ?s then _ else _] |- _ =>
             let b := fresh in
             let Heqb := fresh in
-            remember (Id.FSet.mem x s) as b eqn:Heqb;
+            remember (VarSet.mem x s) as b eqn:Heqb;
             symmetry in Heqb;
             destruct b;
-            [| apply Id.FSetProperties.Dec.F.not_mem_iff in Heqb ]
+            [| apply VarSet.Dec.F.not_mem_iff in Heqb ]
         | H : context [option_map _ (unify_aux ?c)] |- _ =>
             let o := fresh in
             let Heqo := fresh in
@@ -187,40 +184,45 @@ Proof.
             destruct o; [ simpl in H; inversion H; subst |]
         | H : Some ?s = unify_aux ?c |- _ =>
             assert (unifies (fold_right
-              (fun p s x => Types.subst s (Types.subst_single (fst p) (snd p) x))
+              (fun p s x => (Types.subst_single (fst p) (snd p) x).[s])
               Types.Var s) c) by
               (apply IHc; [| rewrite <- H ]; eauto);
             clear H
         | H : Forall _ (_ :: _) |- _ => inversion H; clear H; subst
         | |- Forall _ (_ :: _) => constructor
-        | H : Forall _ (map _ _) |- _ => apply Forall_map in H
+        | H : unifies _ _.|[_] |- _ => generalize (proj1 (Forall_map _ _ _ _ _) H); simpl; intros; clear H
         | H : Forall _ ?l |- Forall _ ?l =>
             eapply Forall_impl; [| apply H ];
             intros
         end;
         repeat (simpl in *; match goal with
-        | H : ~Id.FSet.In ?x (Id.FSet.union ?s1 ?s2) |- _ =>
-            assert (~Id.FSet.In x s1) by eauto;
-            assert (~Id.FSet.In x s2) by eauto;
+        | H : ~VarSet.In ?x (VarSet.union ?s1 ?s2) |- _ =>
+            assert (~VarSet.In x s1) by eauto;
+            assert (~VarSet.In x s2) by eauto;
             clear H
-        | _ => rewrite Types.subst_subst in *
+        | H : context [_.[_].[_]] |- _ => rewrite subst_comp in H
+        | |- context [_.[_].[_]] => rewrite subst_comp
         | |- context [Types.subst_single] => unfold Types.subst_single
         | H : context [Types.subst_single] |- _ => unfold Types.subst_single in *
-        | |- context [Id.eq_dec ?x ?y] => destruct (Id.eq_dec x y)
+        | |- context [scomp] => unfold scomp
+        | H : context [scomp] |- _ => unfold scomp in H
+        | |- context [funcomp] => unfold funcomp
+        | H : context [funcomp] |- _ => unfold funcomp in H
+        | |- context [Nat.eq_dec ?x ?y] => destruct (Nat.eq_dec x y)
         end); simpl in *; try congruence.
       * f_equal; apply Types.subst_ext; intros;
-          destruct (Id.eq_dec t0 x); simpl; congruence.
+          destruct (Nat.eq_dec v x); simpl; congruence.
       * f_equal; apply Types.subst_ext; intros;
-          destruct (Id.eq_dec t0 x); simpl; congruence.
+          destruct (Nat.eq_dec v x); simpl; congruence.
 Qed.
 
 Notation moregen s s' :=
-  (exists s0, forall e, Types.subst s e = Types.subst s0 (Types.subst s' e)).
+  (exists s0, forall e, e.[s] = e.[s'].[s0]).
 
 Lemma subst_single_preserves_unifies : forall x t0 s c,
-  s x = Types.subst s t0 ->
+  s x = t0.[s] ->
   unifies s c ->
-  unifies s (subst (Types.subst_single x t0) c).
+  unifies s (c.|[Types.subst_single x t0]).
 Proof.
   intros ? ? ? ? ? H.
   apply Forall_map.
@@ -232,15 +234,16 @@ Qed.
 Hint Resolve subst_single_preserves_unifies.
 
 Lemma moregen_extend : forall s x t s',
-  s x = Types.subst s t ->
+  s x = t.[s] ->
   moregen s s' ->
-  moregen s (fun y => Types.subst s' (Types.subst_single x t y)).
+  moregen s (fun y => (Types.subst_single x t y).[s']).
 Proof.
   intros ? ? ? ? ? H.
   destruct H as [s'' H].
   exists s''.
   intros.
-  rewrite <- Types.subst_subst.
+  replace (e.[fun y : var => (Types.subst_single x t0 y).[s']])
+    with (e.[Types.subst_single x t0].[s']) by autosubst.
   rewrite <- H.
   rewrite Types.subst_single_preserves_unifies; eauto.
 Qed.
@@ -258,8 +261,7 @@ Proof.
     split; eauto.
     eexists s.
     intros.
-    rewrite Types.subst_id.  
-    eauto.
+    autosubst.
   - destruct (Types.eq_dec t1 t2).
     + subst.
       inversion Hunifies.
@@ -268,20 +270,20 @@ Proof.
       simpl in *.
       destruct t1; destruct t2;
         repeat match goal with
-        | |- context [Id.FSet.mem ?x ?s] =>
+        | |- context [VarSet.mem ?x ?s] =>
             let b := fresh in
             let Heqb := fresh in
-            remember (Id.FSet.mem x s) as b eqn:Heqb;
+            remember (VarSet.mem x s) as b eqn:Heqb;
             symmetry in Heqb;
             destruct b;
-            [ apply Id.FSet.mem_spec in Heqb;
+            [ apply VarSet.mem_spec in Heqb;
               exfalso;
               eapply Types.unifies_occur; eauto
-            | apply Id.FSetProperties.Dec.F.not_mem_iff in Heqb ]
+            | apply VarSet.Dec.F.not_mem_iff in Heqb ]
         | |- context [unify_aux ?c] =>
             assert (H : exists s', option_map (fold_right
-              (fun p s x => Types.subst s (Types.subst_single (fst p) (snd p) x)) Types.Var)
-              (unify_aux c) = Some s' /\ moregen s s');
+              (fun p s x => (Types.subst_single (fst p) (snd p) x).[s])
+              Types.Var) (unify_aux c) = Some s' /\ moregen s s');
             [ apply IHc; eauto
             | destruct H as [? [H]];
               let o := fresh in
@@ -303,7 +305,7 @@ Proof.
 Qed.
 
 Definition unify' : forall c,
-  { s | unifies s c /\ (forall s', unifies s' c -> moregen s' s) } + { forall s, ~unifies s c }.
+  { s | unifies s c /\ (forall s', unifies s' c -> moregen s' s) } + {(forall s, ~unifies s c)}.
 Proof.
   intros c.
   remember (unify c) as o.
