stlc/Types.v
@@ -1,41 +1,32 @@
+Require Import Autosubst.Autosubst.
 Require Import List Omega.
-Require Id.
+Require VarSet.
 
 Inductive t :=
-  | Bool
   | Fun : t -> t -> t
-  | Var : Id.t -> t.
+  | Var : var -> t.
+
+Instance Ids_t : Ids t. derive. Defined.
+Instance Rename_t : Rename t. derive. Defined.
+Instance Subst_t : Subst t. derive. Defined.
+Instance SubstLemmas_t : SubstLemmas t. derive. Qed.
 
 Fixpoint FV t :=
   match t with
-  | Bool => Id.FSet.empty
-  | Fun t1 t2 => Id.FSet.union (FV t1) (FV t2)
-  | Var x => Id.FSet.singleton x
+  | Fun t1 t2 => VarSet.union (FV t1) (FV t2)
+  | Var x => VarSet.singleton x
   end.
 
 Fixpoint size t :=
   match t with
-  | Bool => 1
   | Fun t1 t2 => 1 + size t1 + size t2
   | Var _ => 1
-  end.
-
-Fixpoint subst s t :=
-  match t with
-  | Bool => Bool
-  | Fun t1 t2 => Fun (subst s t1) (subst s t2)
-  | Var x => s x
   end.
 
 Definition eq_dec : forall t1 t2 : t, { t1 = t2 } + { t1 <> t2 }.
 Proof.
   refine (fix eq_dec t1 t2 :=
     match t1 as t1_ return { t1_ = t2 } + { t1_ <> t2 } with
-    | Bool =>
-        match t2 with
-        | Bool => left _
-        | _ => right _
-        end
     | Fun t11 t12 =>
         match t2 with
         | Fun t21 t22 =>
@@ -48,7 +39,7 @@ Proof.
     | Var x =>
         match t2 with
         | Var y =>
-            if Id.eq_dec x y then left _
+            if eq_nat_dec x y then left _
             else right _
         | _ => right _
         end
@@ -63,66 +54,51 @@ Proof.
 Qed.
 
 Lemma subst_FV : forall x s t,
-  Id.FSet.In x (FV (subst s t)) ->
-  exists y, Id.FSet.In x (FV (s y)) /\ Id.FSet.In y (FV t).
+  VarSet.In x (FV t.[s]) ->
+  exists y, VarSet.In x (FV (s y)) /\ VarSet.In y (FV t).
 Proof.
   intros x s t H.
   induction t; simpl in *; eauto.
-  - destruct (Id.FSet.empty_spec H).
-  - apply Id.FSet.union_spec in H.
+  - apply VarSet.union_spec in H.
     destruct H as [H | H];
     [ destruct (IHt1 H) as [? []]
     | destruct (IHt2 H) as [? []]];
     eauto.
 Qed.
 
-Lemma subst_id : forall t, subst Var t = t.
-Proof.
-  intros t.
-  induction t; simpl in *; congruence.
-Qed.
-
 Lemma subst_ext : forall s s' t,
-  (forall x, Id.FSet.In x (FV t) -> s x = s' x) ->
-  subst s t = subst s' t.
+  (forall x, VarSet.In x (FV t) -> s x = s' x) ->
+  t.[s] = t.[s'].
 Proof.
   intros ? ? t ?.
   induction t; simpl in *; f_equal; eauto.
 Qed.
 
-Lemma subst_subst : forall s s' t,
-  subst s (subst s' t) = subst (fun x => subst s (s' x)) t.
-Proof.
-  intros ? ? t.
-  induction t; simpl in *; f_equal; eauto.
-Qed.
-
 Lemma unifies_occur : forall x t,
-  Var x <> t -> Id.FSet.In x (FV t) -> forall s, s x <> subst s t.
+  Var x <> t -> VarSet.In x (FV t) -> forall s, s x <> t.[s].
 Proof.
   intros x t ? ? s Hunifies.
-  assert (Hsize : size (subst s t) <= size (s x)) by (rewrite Hunifies; omega).
+  assert (Hsize : size t.[s] <= size (s x)) by (rewrite Hunifies; omega).
   clear Hunifies.
   induction t; simpl in *.
-  - destruct (Id.FSet.empty_spec H0).
-  - apply Id.FSet.union_spec in H0.
+  - apply VarSet.union_spec in H0.
     destruct H0; [ apply IHt1 | apply IHt2 ];
       try (intros Hcontra; rewrite <- Hcontra in *; simpl in *);
       solve [ omega | eauto ].
-  - apply Id.FSet.singleton_spec in H0.
+  - apply VarSet.singleton_spec in H0.
     congruence.
 Qed.
 
 Definition subst_single x t1 y :=
-  if Id.eq_dec x y then t1
+  if eq_nat_dec x y then t1
   else Var y.
 
 Lemma subst_single_preserves_unifies : forall x t0 s t,
-  s x = subst s t0 ->
-  subst s (subst (subst_single x t0) t) = subst s t.
+  s x = t0.[s] ->
+  t.[subst_single x t0].[s] = t.[s].
 Proof.
   intros ? ? ? t ?.
   induction t; simpl in *; f_equal; eauto.
   unfold subst_single.
-  destruct (Id.eq_dec x t1); subst; eauto.
+  destruct (Nat.eq_dec x v); subst; eauto.
 Qed.
