stlc/Normalization.v
@@ -1,0 +1,115 @@
+Require Import Autosubst.Autosubst.
+Require Types Term.
+Require Import Reduction Typing.
+
+Notation SN e :=
+  (Acc (fun e e' => red e' e) e).
+
+Fixpoint reducible e t : Prop :=
+  match t with
+  | Types.Var _ => SN e
+  | Types.Fun t1 t2 =>
+      forall v, reducible v t1 -> reducible (Term.App e v) t2
+  end.
+Hint Constructors Acc.
+
+Notation neutral t := match t with Term.Abs _ _ => False | _ => True end.
+
+Lemma CR2 t : forall e e',
+  red e e' ->
+  reducible e t -> reducible e' t.
+Proof.
+  induction t; intros ? ? ? Hreducible; simpl in *; eauto.
+  - inversion Hreducible; eauto.
+Qed.
+Hint Resolve CR2.
+
+Lemma CR1_CR3 t :
+  (forall e, reducible e t -> SN e) /\
+  (forall e, neutral e ->
+    (forall e', red e e' -> reducible e' t) -> reducible e t).
+Proof.
+  induction t; split; simpl in *; eauto.
+  - intros ? H.
+    destruct IHt1 as [ IHt1C1 IHt1C3 ].
+    assert (Hc : reducible (Term.Var 0) t1).
+    { apply IHt1C3; eauto.
+      intros ? Hred.
+      inversion Hred. }
+    apply H in Hc.
+    destruct IHt2 as [ IHt2C1 ].
+    apply IHt2C1 in Hc.
+    clear H.
+    remember (Term.App e (Term.Var 0)) as e'.
+    generalize dependent e.
+    induction Hc; intros; subst.
+    eauto.
+  - intros ? Hneutral H ? HRt1.
+    destruct IHt1 as [ IHt1C1 IHt1C3 ].
+    destruct IHt2 as [ IHt2C1 IHt2C3 ].
+    apply IHt2C3; eauto.
+    specialize (IHt1C1 _ HRt1).
+    induction IHt1C1.
+    intros ? Hred.
+    inversion Hred; subst; eauto.
+    inversion Hneutral.
+Qed.
+
+Let CR1 t := proj1 (CR1_CR3 t).
+Let CR3 t := proj2 (CR1_CR3 t).
+Hint Resolve CR1.
+
+Lemma reducible_abs : forall e1 t1 t2,
+  (forall v, reducible v t1 -> reducible (e1.[v/]) t2) ->
+  reducible (Term.Abs t1 e1) (Types.Fun t1 t2).
+Proof.
+  simpl.
+  intros ? ? ? Hsubst ? Hreducible.
+  generalize (CR1 _ _ Hreducible). intros HSN.
+  generalize (CR1 _ _ (Hsubst _ Hreducible)). intros HSNsubst.
+  generalize dependent e1.
+  induction HSN as [? ? IH].
+  intros.
+  remember (e1.[x/]) as e.
+  generalize dependent e1.
+  generalize dependent x.
+  induction HSNsubst as [? ? IH'].
+  intros. subst.
+  apply CR3; eauto.
+  intros ? Hred.
+  inversion Hred; subst; eauto 7.
+  inversion H4; subst.
+  eapply IH'; try reflexivity; eauto.
+Qed.
+
+Lemma fundamental_property env t T :
+  typed env t T ->
+  forall s,
+  (forall x T, env x = Some T -> reducible (s x) T) ->
+  reducible (t.[s]) T.
+Proof.
+  induction 1; intros ? Hsubst; simpl in *; eauto.
+  - intros ? Hreducible.
+    apply reducible_abs; eauto.
+    intros ? ?.
+    rewrite subst_comp.
+    apply IHtyped.
+    intros [| x] ? Heq; simpl in *.
+    + congruence.
+    + replace ((up s (S x)).[v0/]) with (s x) by autosubst.
+      eauto.
+Qed.
+
+Theorem strong_normalization env t T :
+  typed env t T ->
+  SN t.
+Proof.
+  intros Htyped.
+  apply fundamental_property with (s := ids) in Htyped.
+  - rewrite subst_id in Htyped.
+    eauto.
+  - intros ? ? ?.
+    apply CR3; simpl; eauto.
+    intros ? Hred.
+    inversion Hred.
+Qed.
