stlc/Reduction.v
@@ -1,0 +1,33 @@
+Require Import Autosubst.Autosubst.
+Require Import Arith List Program Omega Relations.
+Require Term Types.
+
+Inductive red : Term.t -> Term.t -> Prop :=
+  | R_Abs : forall t e e',
+      red e e' ->
+      red (Term.Abs t e) (Term.Abs t e')
+  | R_AppL : forall e1 e1' e2,
+      red e1 e1' ->
+      red (Term.App e1 e2) (Term.App e1' e2)
+  | R_AppR : forall e1 e2 e2',
+      red e2 e2' ->
+      red (Term.App e1 e2) (Term.App e1 e2')
+  | R_Red : forall t e e2,
+      red (Term.App (Term.Abs t e) e2) (e.[e2/]).
+Hint Constructors red clos_refl_trans.
+
+Lemma ered_appabs T t11 t2 t :
+  t = t11.[t2/] ->
+  red (Term.App (Term.Abs T t11) t2) t.
+Proof. intros. subst. econstructor. Qed.
+
+Lemma red_subst t t' :
+  red t t' ->
+  forall s,
+  red t.[s] t'.[s].
+Proof.
+  induction 1; simpl; intros ?; eauto.
+  - apply ered_appabs.
+    autosubst.
+Qed.
+Hint Resolve red_subst.
