stlc/Term.v
@@ -1,0 +1,27 @@
+Require Import Autosubst.Autosubst.
+Require Import Arith List Omega Program.
+Require Types.
+
+Inductive t :=
+  | Var (x : var)
+  | Abs (T : Types.t) (s : {bind t})
+  | App (t1 t2 : t).
+
+Fixpoint FTV e :=
+  match e with
+  | Var _ => VarSet.empty
+  | Abs t e => VarSet.union (Types.FV t) (FTV e)
+  | App e1 e2 => VarSet.union (FTV e1) (FTV e2)
+  end.
+
+Instance Ids_t : Ids t. derive. Defined.
+Instance Rename_t : Rename t. derive. Defined.
+Instance Subst_t : Subst t. derive. Defined.
+Instance SubstLemmas_t : SubstLemmas t. derive. Qed.
+Instance HSubst_t : HSubst Types.t t. derive. Defined.
+Instance HSubstLemmas_t : HSubstLemmas Types.t t. derive. Defined.
+Instance SubstHSubstComp_t : SubstHSubstComp Types.t t. derive. Defined.
+
+Inductive value : t -> Prop :=
+  | V_Abs : forall e t, value (Abs t e).
+Hint Constructors value.
