stlc/TypeSafety.v
@@ -1,42 +1,19 @@
+Require Import Autosubst.Autosubst.
 Require Import List Relations Program.
-Require Import Id Types Exp SmallstepCbv Typing.
+Require Types Term Reduction Typing.
 
-Lemma preservation : forall e e',
-  simplto e e' ->
+Lemma preservation e e' :
+  Reduction.red e e' ->
   forall env t,
-  typed env e t ->
-  typed env e' t.
+  Typing.typed env e t ->
+  Typing.typed env e' t.
 Proof.
-  intros ? ? Hsimplto.
-  induction Hsimplto; intros ? ? Htyped; inversion Htyped; eauto.
+  induction 1; intros ? ? Htyped; inversion Htyped; subst; eauto.
 
-  inversion H3.
-  eapply substitution with (env' := []); eauto.
-  reflexivity.
+  inversion H2; subst.
+  eapply Typing.typed_subst; eauto.
+  intros [| ?] ? Heq; simpl in *.
+  - congruence.
+  - eauto.
 Qed.
-
-Lemma progress : forall e t,
-  typed [] e t ->
-  value e \/ exists e', simplto e e'.
-Proof.
-  intros ? ? Htyped.
-  remember [] as env.
-  induction Htyped; subst; simpl in *; eauto.
-  - destruct x; congruence.
-  - destruct (IHHtyped1 eq_refl) as [ H | []]; [| eauto ].
-    destruct (canonical_form_fun _ _ _ H Htyped1); subst.
-    destruct (IHHtyped2 eq_refl) as [| []]; eauto.
-Qed.
-
-Theorem type_safety : forall e e',
-  clos_refl_trans _ simplto e e' ->
-  forall t,
-  typed [] e t ->
-  value e' \/ exists e'', simplto e' e''.
-Proof.
-  intros ? ? H.
-  apply clos_rt_rt1n in H.
-  Hint Resolve preservation progress.
-  induction H; intros ? Htyped; eauto.
-Qed.
-
+    
