stlc/VarSet.v
@@ -1,0 +1,29 @@
+Require Import Autosubst.Autosubst.
+Require Import Arith MSets.
+
+Module VarSet := MSetList.Make (Nat_as_OT).
+Include VarSet.
+Include (WProperties (VarSet)).
+
+Definition fresh s :=
+  match max_elt s with
+  | None => 0
+  | Some n => S n
+  end.
+
+Lemma fresh_spec : forall s, ~ In (fresh s) s.
+Proof.
+  unfold fresh.
+  intros s ?.
+  remember (max_elt s) as m.
+  symmetry in Heqm.
+  destruct m.
+  - eapply max_elt_spec2; eauto.
+  - apply max_elt_spec3 in Heqm.
+    destruct (Heqm _ H).
+Qed.
+
+Hint Extern 1 (In _ (union _ _)) =>
+  apply union_spec.
+Hint Extern 1 (In _ (singleton _)) =>
+  apply singleton_spec.
